examples/scache/AtomicIndexLookup.i.dfy
@@ -30,6 +30,9 @@ module AtomicIndexLookupImpl {
     forall v, g :: atomic_inv(a, v, g) <==> state_inv(v, g, disk_idx)
   }
 
+  method unsafe_obtain<Q>() returns (linear r: Q)
+  method unsafe_dispose<Q>(linear r: Q)
+
   method atomic_index_lookup_read(
       a: AtomicIndexLookup,
       disk_idx: int)
@@ -39,17 +42,62 @@ module AtomicIndexLookupImpl {
 
   method atomic_index_lookup_add_mapping(
       a: AtomicIndexLookup,
-      disk_idx: int,
-      cache_idx: int,
-      linear m: CacheResources.R)
+      disk_idx: uint64,
+      cache_idx: uint64,
+      linear cache_entry: CacheResources.R,
+      linear status: CacheResources.R)
   returns (
     success: bool,
-    linear m': CacheResources.R
+    linear cache_entry': CacheResources.R,
+    linear status': CacheResources.R,
+    linear read_ticket: maybe<CacheResources.R>
   )
-  requires m.CacheEntry?
-  requires m.disk_idx_opt == None
-  requires m.cache_idx == cache_idx
-  ensures !success ==> m' == m
-  ensures success ==> m' == m.(disk_idx_opt := Some(disk_idx))
+  requires atomic_index_lookup_inv(a, disk_idx as int)
+  requires cache_entry.CacheEntry?
+  requires cache_entry.disk_idx_opt == None
+  requires cache_entry.cache_idx == cache_idx as int
+  requires status == CacheStatus(cache_idx as int, Empty)
+  requires 0 <= cache_idx as int < CACHE_SIZE
+  ensures !success ==> cache_entry' == cache_entry
+  ensures success ==> cache_entry' ==
+      cache_entry.(disk_idx_opt := Some(disk_idx as int))
+  ensures !success ==> status' == status
+  ensures success ==> status' == CacheStatus(cache_idx as int, Reading)
+  ensures success ==> has(read_ticket)
+      && read(read_ticket) == DiskReadTicket(disk_idx)
+  ensures !success ==> !has(read_ticket)
+  {
+    var did_set := compare_and_set(a, NOT_MAPPED, cache_idx);
 
+    ///// Begin jank
+    ///// Setup:
+    var v1 := NOT_MAPPED;
+    var v2 := cache_idx;
+    var old_v: uint64;
+    var new_v: uint64;
+    linear var old_g: CacheResources.R := unsafe_obtain();
+    assume old_v == v1 ==> new_v == v2 && did_set;
+    assume old_v != v1 ==> new_v == old_v && !did_set;
+    assume atomic_inv(a, old_v, old_g);
+    linear var new_g;
+    ///// Transfer:
+    if did_set {
+      linear var ticket;
+      status', cache_entry', new_g, ticket :=
+        initiate_page_in(cache_idx as int, disk_idx, status, cache_entry, old_g);
+      read_ticket := give(ticket);
+    } else {
+      cache_entry' := cache_entry;
+      status' := status;
+      read_ticket := empty();
+      new_g := old_g;
+    }
+    assert state_inv(new_v, new_g, disk_idx as int);
+    ///// Teardown:
+    assert atomic_inv(a, new_v, new_g);
+    unsafe_dispose(new_g);
+    ///// End jank
+
+    success := did_set;
+  }
 }
