examples/scache/CacheResources.i.dfy
@@ -7,7 +7,55 @@ module CacheResources refines ResourceSpec {
   import opened Options
   import opened NativeTypes
 
+  datatype Status = Empty | Reading | Clean | Dirty | WriteBack
+
   datatype R =
     | DiskPageMap(disk_idx: int, cache_idx_opt: Option<int>)
-    | CacheEntry(disk_idx_opt: Option<int>, cache_idx: int, data: seq<byte>)
+    | CacheEntry(disk_idx_opt: Option<int>,
+        cache_idx: int, data: seq<byte>)
+
+    | CacheStatus(cache_idx: int, status: Status)
+
+    | DiskReadTicket(addr: uint64)
+    | DiskReadStub(addr: uint64, contents: seq<byte>)
+
+  method initiate_page_in(
+      cache_idx: int,
+      disk_idx: uint64,
+      linear s1: R,
+      linear s2: R,
+      linear s3: R
+  )
+  returns (
+      linear t1: R,
+      linear t2: R,
+      linear t3: R,
+      linear t4: R
+  )
+  requires s1 == CacheStatus(cache_idx, Empty)
+  requires s2.CacheEntry? && s2.cache_idx == cache_idx
+      && s2.disk_idx_opt == None
+  requires s3 == DiskPageMap(disk_idx as int, None)
+  ensures t1 == CacheStatus(cache_idx, Reading)
+  ensures t2 == s2.(disk_idx_opt := Some(disk_idx as int))
+  ensures t3 == DiskPageMap(disk_idx as int, Some(cache_idx))
+  ensures t4 == DiskReadTicket(disk_idx)
+
+  method finish_page_in(
+      cache_idx: int,
+      disk_idx: uint64,
+      linear s1: R,
+      linear s2: R,
+      linear s3: R
+  )
+  returns (
+      linear t1: R,
+      linear t2: R
+  )
+  requires s1 == CacheStatus(cache_idx, Reading)
+  requires s2.CacheEntry? && s2.disk_idx_opt == Some(disk_idx as int)
+      && s2.cache_idx == cache_idx
+  requires s3.DiskReadStub? && s3.addr == disk_idx
+  ensures t1 == CacheStatus(cache_idx, Clean)
+  ensures t2 == s2.(data := s3.contents)
 }
